thys/AutoCorres2/tests/c-parser/arithmetic_right_shift.c
@@ -1,0 +1,20 @@
+/*
+ * Copyright (c) 2024 Apple Inc. All rights reserved.
+ *
+ * SPDX-License-Identifier: BSD-2-Clause
+ */
+
+int c;
+unsigned u;
+
+int f(void)
+{
+  c = c >> 5;
+  return c;
+}
+
+unsigned g(void)
+{
+  u = u >> 5;
+  return u;
+}
