thys/AutoCorres2/tests/c-parser/padding_free.c
@@ -1,0 +1,37 @@
+typedef unsigned char  uint8_t;
+typedef unsigned short uint16_t;
+typedef unsigned int   uint32_t;
+
+typedef struct {
+  uint8_t field1;
+  uint8_t pad1;
+  uint16_t field2;
+  uint16_t pad2;
+  uint8_t field3;
+  uint8_t field4;
+  uint32_t pad3;
+} p_t;
+
+typedef struct {
+  uint16_t field1;
+  uint16_t pad1;
+  uint32_t field2;
+} q_t;
+
+typedef struct {
+  uint32_t field1;
+  uint16_t pad1;
+  uint16_t field2;
+} r_t;
+
+uint8_t f(p_t p) {
+  return p.field1;
+}
+
+uint16_t g(q_t q) {
+  return q.field1;
+}
+
+uint32_t h(r_t r) {
+  return r.field1;
+}
