thys/AutoCorres2/tests/proof-tests/anonymous_nested_struct.c
@@ -1,0 +1,36 @@
+/*
+ * Copyright (c) 2025 Apple Inc. All rights reserved.
+ *
+ * SPDX-License-Identifier: BSD-2-Clause
+ */
+
+typedef struct {
+  unsigned char id;
+  union {
+    struct {
+      int x;
+      int y;
+    };
+    struct {
+      int r;
+      int phi;
+    };
+  };
+} coord_t;
+
+int main (coord_t x) {
+  x.phi = 2;
+  x.x = 1;
+  return x.r;
+}
+
+typedef struct {
+  int fst;
+  int snd;
+} pair_t;
+
+int foo (void) {
+  int o1 = __builtin_offsetof(pair_t, fst);
+  int o2 = __builtin_offsetof(coord_t, x);
+  return o1;
+}
