thys/AutoCorres2/tests/proof-tests/fnptr_no_heap_abs.c
@@ -1,0 +1,72 @@
+/*
+ * Copyright (c) 2024 Apple Inc. All rights reserved.
+ *
+ * SPDX-License-Identifier: BSD-2-Clause
+*/
+
+typedef char  (*object_f1_t)(unsigned long object);
+typedef short (*object_f2_t)(unsigned long object);
+typedef int   (*object_f3_t)(unsigned long object);
+
+typedef struct {
+    object_f1_t f1_ptr;
+    object_f2_t f2_ptr;
+    object_f3_t f3_ptr;
+} obj_fnptr_t;
+
+typedef struct {
+    char  c1;
+    short s1;
+    int   i1;
+} obj1_t;
+
+typedef struct {
+    short s2;
+    int   i2;
+    char  c2;
+} obj2_t;
+
+#define ptr(x) ((void *) x)
+
+char
+obj1_f1(unsigned long object) {
+    obj1_t *obj = ptr(object);
+    return obj->c1;
+}
+
+short
+obj1_f2(unsigned long object) {
+    obj1_t *obj = ptr(object);
+    return obj->s1;
+}
+
+int
+obj1_f3(unsigned long object) {
+    obj1_t *obj = ptr(object);
+    return obj->i1;
+}
+
+char
+obj2_f1(unsigned long object) {
+    obj2_t *obj = ptr(object);
+    return obj->c2;
+}
+
+static const obj_fnptr_t array[] =
+  {
+    {
+        .f1_ptr = obj1_f1, .f2_ptr = obj1_f2, .f3_ptr = obj1_f3
+    },
+    {
+       .f1_ptr = obj2_f1, .f2_ptr = 0, .f3_ptr = 0
+    }
+  };
+
+char
+f1(unsigned short type, unsigned long x) {
+    if (array[type].f1_ptr != 0) {
+        return (char) array[type].f1_ptr(x);
+    } else {
+        return 1;
+    }
+}
