thys/AutoCorres2/tests/proof-tests/in_out_parameters_no_hl.c
@@ -1,0 +1,37 @@
+/*
+ * Copyright (c) 2023 Apple Inc. All rights reserved.
+ *
+ * SPDX-License-Identifier: BSD-2-Clause
+ */
+
+
+typedef struct pair {
+unsigned fst;
+unsigned snd;
+} pair_t;
+
+
+unsigned get_fst(pair_t p, pair_t *q) {
+ if (p.fst == 0) {
+   exit (1);
+ } else {
+   q -> fst = p.snd;
+   q -> snd = p.fst;
+   return (q->fst);
+ }
+}
+
+pair_t * g;
+
+unsigned main(unsigned n, unsigned m) {
+  unsigned n1 = n;
+  unsigned m1 = n;
+  pair_t local_p;
+  local_p.fst = n;
+  local_p.snd = m;
+  m1 = get_fst(local_p, g);
+  return m + n + n1 + m1;
+}
+
+
+
