thys/AutoCorres2/tests/proof-tests/side_effect_assignment.c
@@ -1,0 +1,127 @@
+/*
+ * Copyright (c) 2025 Apple Inc. All rights reserved.
+ *
+ * SPDX-License-Identifier: BSD-2-Clause
+ */
+
+unsigned main(unsigned n, unsigned *q) {
+  unsigned * p = q;
+  *(p++) = n;
+  *p = n + 1;
+  *(p--) = n + 1;
+  return (*p);
+}
+
+unsigned main1(unsigned n, unsigned *q) {
+  unsigned * p = q;
+  *(p + 1) = n;
+  *p = n + 1;
+  return (*p);
+}
+
+
+
+void foo(unsigned  * p) {
+  *(p++) = 0;
+}
+
+unsigned arr[120];
+
+unsigned add (unsigned x, unsigned y) {
+  return (x + y);
+}
+
+unsigned arr_upd(unsigned i, unsigned v) {
+  arr[i++] = add(v, v);
+  arr[v] = i++;
+  while (add(v,i) ) {
+    arr[i] = i;
+  }
+  while (add(v--,i) ) {
+    arr[i] = i;
+  }
+  while (add(v--,i) ) {
+    if (i < 2) break;
+    arr[i] = i;
+  }
+  while (add(v--,i) ) {
+    if (i < 2) continue;
+    arr[i] = i;
+  }
+  while (add(v--,i) ) {
+    if (i < 2) return 42;
+    if (i < 3) goto cleanup;
+    arr[i] = i;
+  }
+cleanup:
+  return v;
+}
+
+unsigned loop1(unsigned n) {
+  unsigned m = 0;
+  while (n--) {
+    m++;
+  }
+  return m;
+}
+
+unsigned loop2(unsigned n) {
+  unsigned m = 0;
+  while (1) {
+    if (n) {n--;} else {n--; break;};
+    m++;
+  }
+  return m;
+}
+
+unsigned main2(unsigned n) {
+  unsigned m = 0;
+  unsigned x = 0;
+  for (unsigned i = 0; i < 120; i++) {
+    arr[i] = n++ + m++;
+    x = m;
+  }
+
+  while (1) {
+    x--;
+  }
+
+  while (n--) {
+    m++;
+  }
+  return m;
+}
+
+unsigned main3(unsigned n) {
+  unsigned m = 0;
+  unsigned x = 0;
+  for (unsigned i = 0; i < 120; i++) {
+    arr[i] = n++ + m++;
+    x = m;
+  }
+  while (n--) {
+    m++;
+  }
+
+  return m;
+}
+
+
+/* FIXME: abstract_try_catch fails here */
+/*
+unsigned main4(unsigned n) {
+  unsigned m = 0;
+  unsigned x = 0;
+
+  while (1) {
+    if (n) {n--;} else {n--; break;};
+    m++;
+  };
+
+  while (1) {
+    x--;
+  }
+  return m;
+}
+*/
+
