thys/AutoCorres2/tests/proof-tests/struct_consecutive_init.c
@@ -115,3 +115,220 @@ int string_of_vars_explode(int n, int m, int k) {
     return n5;
 };
 
+void crosswise_init() {
+  unsigned i;
+  POINT src, dst;
+
+ for(i = 0; i <= 2; i++ ) {
+    src.a = 33;
+    dst.a = 42;
+    src.b = 8;  
+    dst.b = 8;
+  }
+
+  return;
+}
+
+POINT cond_init(unsigned i) {
+  POINT src;
+  src.a = 33;
+  if (i < 42) {
+    src.b = 44;
+  } else {
+    src.b = 42;
+  }
+  return src;
+}
+
+POINT cond_init1(unsigned i) {
+  POINT src;
+  if (i < 42) {
+    src.b = 44;
+  } else {
+    src.b = 42;
+  }
+  src.a = 33;
+  return src;
+}
+
+POINT swap (POINT p) {
+  return (POINT) {p.b, p.a};
+};
+
+unsigned cond_init_while (unsigned i) {
+  POINT src;
+  POINT dst;
+  unsigned x = 0;
+  while (i < 100) {
+    if (i < 42) {
+      src.a = i + 2;
+      dst.a = i + 3;
+    } else {
+      src.a = i + 3;
+      dst.a = x + 2;
+    }
+    src.b = i;
+    dst.b = i;
+    x = x + i + src.a + dst.b + src.b + dst.a;
+    i = i + 1;
+  }
+  return (x);
+}
+
+unsigned cond_init_while_nested (unsigned i) {
+  POINT src;
+  LINE dst;
+  unsigned x = 0;
+  while (i < 100) {
+    if (i < 42) {
+      src.a = i + 2;
+      dst.from.a = i + 3;
+      dst.to.a = i + 4;
+    } else {
+      src.a = i + 3;
+      dst.from.a = i + 4;
+      dst.to.a = i + 5;
+    }
+    src.b = i;
+    dst.from.b = i;
+    dst.to.b = i;
+    x = x + i + src.a + dst.from.a + dst.from.b + src.b + dst.to.a + dst.to.b;
+    i = i + 1;
+  }
+  return (x);
+}
+
+unsigned cond_init_while_incomplete (unsigned i) {
+  POINT src;
+  POINT dst;
+  unsigned x = 0;
+  while (i < 100) {
+    if (i < 42) {
+      src.a = i + 2;
+      dst.a = i + 3;
+    } else {
+      src.a = i + 3;
+      dst.a = x + 2;
+    }
+    src.b = i;
+
+    x = x + i + src.a + dst.b + src.b + dst.a;
+    i = i + 1;
+  }
+  return (x);
+}
+
+unsigned cond_init_while3 (unsigned i) {
+  POINT src;
+  POINT dst;
+  POINT three;
+  unsigned x = 0;
+  while (i < 100) {
+    if (i < 42) {
+      src.a = i + 2;
+      dst.a = i + 3;
+      three.a = i + 4;
+    } else {
+      src.a = i + 3;
+      dst.a = x + 2;
+      three.a = i + 5;
+    }
+    src.b = i;
+    dst.b = i;
+    three.b = i;
+    x = x + i + src.a + dst.b + src.b + dst.a + three.a + three.b;
+    i = i + 1;
+  }
+  return (x);
+}
+
+unsigned cond_init_while4 (unsigned i) {
+  POINT src;
+  POINT dst;
+  POINT three;
+  POINT four;
+  unsigned x = 0;
+  while (i < 100) {
+    if (i < 42) {
+      src.a = i + 2;
+      dst.a = i + 3;
+      three.a = i + 4;
+      four.a = i + 6;
+    } else {
+      src.a = i + 3;
+      dst.a = x + 2;
+      three.a = i + 5;
+      four.a = i + 7;
+    }
+    src.b = i;
+    dst.b = i;
+    three.b = i;
+    four.b = i;
+    x = x + i + src.a + dst.b + src.b + dst.a + three.a + three.b + four.a + four.b;
+    i = i + 1;
+  }
+  return (x);
+}
+
+unsigned cond_explode (unsigned i) {
+  POINT x;
+  unsigned result = 0;
+  if (i > 1) { 
+    x.a = i;
+  } else {
+    x.a = i + 1;
+  }
+
+  if (i > 3) {
+    result = 2;
+  }
+  
+  if (i > 4) {
+    result = 4;
+  };
+  
+  if (i > 5) {
+    result = 5;
+  };
+
+  if (i > 6) {
+    result = 6;
+  };
+
+  x.b = 42;
+
+  if (i > 7) {
+    result = 7;
+  };
+
+  if (i > 8) {
+    result = 8;
+  };
+
+  if (i > 9) {
+    result = 9;
+  };
+
+  if (i > 10) {
+    result = 10;
+  };
+
+
+  if (i > 11) {
+    result = 11;
+  };
+
+
+  if (i > 12) {
+    result = 12;
+  };
+
+
+  if (i > 13) {
+    result = 13;
+  };
+
+  return result + x.a + x.b;
+}
+
+
