thys/AutoCorres2/lib/Simp_Trace.thy
@@ -27,110 +27,221 @@ ML \<open>
 structure Simp_Trace =
 struct
 
+type cumulative_statistics = 
+  {
+    cumulative_time : Time.time,
+    calls : int
+  }
+
+type call_statistics = 
+  { successes : cumulative_statistics, failures : cumulative_statistics }
+
 type trace_statistics =
   {
-    conditional_rules : (Time.time * int) Thm_Name.Table.table,
+    conditional_rules : call_statistics Thm_Name.Table.table,
+    simprocs : call_statistics Symtab.table,
     rules : int Thm_Name.Table.table,
     steps : int,
     max_steps : int,
     depth : int,
-    max_depth : int
+    max_depth : int,
+    do_trace : bool,
+    in_simproc : bool
   }
 
 structure Data = Proof_Data
-( type T = trace_statistics Synchronized.var option
+( 
+  type T = trace_statistics Synchronized.var option
   fun init _ = NONE
 )
 
 val trace_data : Proof.context -> trace_statistics Synchronized.var option = Data.get
 
-fun initial n : trace_statistics =
+fun initial n do_trace : trace_statistics =
   {
     conditional_rules = Thm_Name.Table.empty,
+    simprocs = Symtab.empty,
     rules = Thm_Name.Table.empty,
     steps = 0,
     max_steps = n,
     depth = 0,
-    max_depth = 0
+    max_depth = 0,
+    do_trace = do_trace,
+    in_simproc = false
   }
 
-fun activate n = Data.put (SOME (Synchronized.var "trace_data" (initial n)))
+fun activate n do_trace = Data.put (SOME (Synchronized.var "trace_data" (initial n do_trace)))
 
-fun print ({conditional_rules, rules, steps, max_depth, ...} : trace_statistics) =
+fun call_statistics_ord (x, y:('a * call_statistics)) =
+  (x, y) |> apply2 (snd #> #failures #> #cumulative_time) |> Time.compare
+
+
+fun print_cumulative_statistics txt { cumulative_time = t, calls = n} =
+  if n = 0 then "no " ^ txt else txt ^ ": " ^ 
+  Time.toString t ^ " / " ^ string_of_int n ^ " = " ^
+    Real.fmt (StringCvt.FIX (SOME 3)) (Time.toReal t / Real.fromInt n)
+
+fun print ({conditional_rules, rules, simprocs, steps, max_depth, ...} : trace_statistics) =
   let
     val _ = writeln ("=== SIMP STATISTICS (" ^
       string_of_int steps ^ " steps, " ^ string_of_int max_depth ^ " max depth) ===")
-    val _ = writeln "Conditional Rules:"
+    val _ = writeln "Conditional Rules (sorted in failure time):"
     val _ = conditional_rules |> Thm_Name.Table.dest
-      |> sort (make_ord (fn ((_, (t1, _)), (_, (t2, _))) => Time.< (t2, t1)))
-      |> app (fn (name, (t, c)) =>
-        writeln ("  " ^ Thm_Name.print name ^ ": " ^ Time.toString t ^ " / " ^ string_of_int c ^ " = " ^
-          Real.toString (Time.toReal t / Real.fromInt c)))
+      |> sort (call_statistics_ord #> rev_order)
+      |> app (fn (name, cs) =>
+        writeln ("  " ^ Thm_Name.print name ^ ": " ^ print_cumulative_statistics "failures" (#failures cs) ^
+          " (" ^ print_cumulative_statistics "successes" (#successes cs) ^ ")"))
     val _ = writeln "Rules:"
     val _ = rules |> Thm_Name.Table.dest
       |> sort (make_ord (fn ((_, c1), (_, c2)) => c2 < c1))
       |> app (fn (name, c) => writeln ("  " ^ Thm_Name.print name ^ ": " ^ string_of_int c))
+    val _ = writeln "Simprocs (sorted in failure time):"
+    val _ = simprocs |> Symtab.dest
+      |> sort (call_statistics_ord #> rev_order)
+      |> app (fn (name, cs) =>
+        writeln ("  " ^ name ^ ": " ^ print_cumulative_statistics "failures" (#failures cs) ^
+          " (" ^ print_cumulative_statistics "successes" (#successes cs) ^ ")"))
     val _ = writeln ("======")
   in
     ()
   end
 
-fun trace_apply var {unconditional, rrule, thm, ...} ctxt cont =
-  let
-    val d = Synchronized.value var
-    val _ = #max_steps d <= #steps d andalso error ("simp tracer: max steps reaches")
-    fun store time = Synchronized.change var (fn
-      { conditional_rules, rules, steps, depth, max_steps, max_depth } =>
-      {
-        conditional_rules = (if unconditional then conditional_rules else
-          conditional_rules |>
-          Thm_Name.Table.map_default (#name rrule, (Time.zeroTime, 0))
-            (fn (t, c) => (Time.+ (t, #cpu time), c + 1))),
-        rules = rules |> Thm_Name.Table.map_default (#name rrule, 0) (fn c => c + 1),
-        steps = steps + 1,
-        max_steps = max_steps,
-        depth = depth,
-        max_depth = max_depth
-      }
-    )
-  in
-    Timing.timing (Exn.capture cont) ctxt
-    |> (fn (t, x) => (store t; Exn.release x))
-  end
+fun map_success f ({ successes, failures } : call_statistics) : call_statistics = 
+  { successes = f successes, failures = failures }
+
+fun map_failure f ({ successes, failures } : call_statistics) : call_statistics = 
+  { successes = successes, failures = f failures }
+
+fun incr_cumulative t ({ cumulative_time, calls } : cumulative_statistics) = 
+  { cumulative_time = Time.+ (t, cumulative_time), calls = calls + 1 }
+
+fun incr_call success t = 
+  (if success then map_success else map_failure) (incr_cumulative t)
+
+val zero_cumulative = { cumulative_time = Time.zeroTime, calls = 0 }
+
+val zero_calls = { successes = zero_cumulative, failures = zero_cumulative }
 
 fun map_depth f
-  ({ conditional_rules, rules, steps, depth, max_steps, max_depth} : trace_statistics) :
+  ({ conditional_rules, simprocs, rules, steps, depth, max_steps, max_depth, do_trace, in_simproc} :
+    trace_statistics) :
   trace_statistics =
 let
   val d = f depth
 in
   { conditional_rules = conditional_rules,
+    simprocs = simprocs,
     rules = rules,
     steps = steps,
     depth = d,
     max_depth = if max_depth < d then d else max_depth,
-    max_steps = max_steps }
+    max_steps = max_steps,
+    do_trace = do_trace,
+    in_simproc = in_simproc }
 end
+
+fun map_in_simproc f
+  ({ conditional_rules, simprocs, rules, steps, depth, max_steps, max_depth, do_trace, in_simproc} :
+    trace_statistics) :
+  trace_statistics =
+{ 
+  conditional_rules = conditional_rules,
+  simprocs = simprocs,
+  rules = rules, 
+  steps = steps, 
+  depth = depth, 
+  max_steps = max_steps, 
+  max_depth = max_depth, 
+  do_trace = do_trace, 
+  in_simproc = f in_simproc
+}
+
+fun trace_apply var {unconditional, rrule, ...} ctxt cont =
+  let
+    val d = Synchronized.value var
+    val _ = #max_steps d <= #steps d andalso error ("simp trace: max steps reaches")
+    fun store success time = Synchronized.change var (fn
+      ({ conditional_rules, simprocs, rules, steps, depth, max_steps, max_depth, do_trace,
+         in_simproc } : trace_statistics) =>
+      {
+        conditional_rules = (if unconditional then conditional_rules else
+          conditional_rules |>
+          Thm_Name.Table.map_default (#name rrule, zero_calls) (incr_call success (#cpu time))),
+        simprocs = simprocs,
+        rules = rules |> Thm_Name.Table.map_default (#name rrule, 0) (fn c => c + 1),
+        steps = steps + 1,
+        max_steps = max_steps,
+        depth = depth,
+        max_depth = max_depth,
+        do_trace = do_trace,
+        in_simproc = in_simproc
+      }
+    )
+  in
+    Timing.timing (Exn.capture cont) ctxt
+    |> (fn (t, x) => (store (Exn.is_res x) t; Exn.release x))
+  end
+
+fun trace_simproc var name ctxt cont =
+  let
+    val d = Synchronized.value var
+    val _ = #max_steps d <= #steps d andalso error ("simp trace: max steps reaches")
+    fun store success time = Synchronized.change var (fn
+      ({ conditional_rules, simprocs, rules, steps, depth, max_steps, max_depth, do_trace, in_simproc }  : trace_statistics) =>
+      {
+        conditional_rules = conditional_rules,
+        simprocs = simprocs |>
+          Symtab.map_default (name, zero_calls) (incr_call success (#cpu time)),
+        rules = rules,
+        steps = steps + 1,
+        max_steps = max_steps,
+        depth = depth,
+        max_depth = max_depth,
+        do_trace = do_trace,
+        in_simproc = false
+      }
+    )
+    fun is_success (Exn.Res (SOME _)) = true
+      | is_success _ = false
+    fun set_in_simproc f x =
+      (Synchronized.change var (map_in_simproc (K f)); x)
+  in
+    Timing.timing (Exn.capture
+      (set_in_simproc true #> cont)) ctxt
+    |> (fn (t, x) => (store (is_success x) t; Exn.release x))
+  end
 
 fun increase_depth var ctxt =
   (Synchronized.change var (map_depth (fn d => d + 1)); ctxt)
 
+fun check_trace_data ctxt =
+  case trace_data ctxt of SOME var => 
+    let
+      val d = Synchronized.value var
+    in
+      if #in_simproc d then NONE else SOME var
+    end
+  | NONE => NONE
+
 val trace_ops : Raw_Simplifier.trace_ops = {
   trace_invoke = fn _ => fn ctxt =>
-    (case trace_data ctxt of SOME var => increase_depth var ctxt
+    (case check_trace_data ctxt of SOME var => increase_depth var ctxt
       | NONE => ctxt),
   trace_rrule = fn rule => fn ctxt => fn cont =>
-    case trace_data ctxt of
+    case check_trace_data ctxt of
       SOME var => trace_apply var rule ctxt cont
     | NONE => cont ctxt,
-  trace_simproc = K (K (K NONE))
+  trace_simproc = fn {name, ...} => fn ctxt => fn cont =>
+    case check_trace_data ctxt of
+      SOME var => trace_simproc var name ctxt cont
+    | NONE => cont ctxt
 }
 
-fun wrapper n tac ctxt st =
+fun wrapper n do_trace tac ctxt st =
   let
     val ctxt' = ctxt
-      |> activate n
-      |> Config.put Raw_Simplifier.simp_trace true
+      |> activate n do_trace
+      |> Config.put Raw_Simplifier.simp_trace do_trace
       |> Config.put Raw_Simplifier.simp_trace_depth_limit 4
     val res = Exn.capture (fn () => (tac ctxt' st |> Seq.pull)) ()
     val _ = print (Synchronized.value (the (trace_data ctxt')))
@@ -141,14 +252,11 @@ fun wrapper n tac ctxt st =
     | NONE => Seq.empty
   end
 
-fun wrapper' n tac ctxt = wrapper n (fn ctxt => tac ctxt 1) ctxt
-
-fun wrapper_method method ctxt' (_, thm) =
-  method (ctxt', thm)
-
-fun method_wrapper (n : int option) (m : Proof.context -> Method.method) ctxt : Method.method =
+fun method_wrapper (n : int option) (do_trace : bool) (m : Proof.context -> Method.method) ctxt : 
+  Method.method =
   fn thms => Method.RUNTIME
-    (wrapper (the_default 1000 n) (fn ctxt => wrapper_method (m ctxt thms) ctxt) ctxt)
+    (wrapper (the_default 1000 n) do_trace 
+      (fn ctxt => fn (_, thm) => m ctxt thms (ctxt, thm)) ctxt)
 
 val no_asmN = "no_asm";
 val no_asm_useN = "no_asm_use";
@@ -163,14 +271,22 @@ val simp_options =
   Args.parens Parse.nat >> (fn n => (SOME n, asm_full_simp_tac)) ||
   Scan.succeed (NONE, asm_full_simp_tac));
 
+val no_traceN = "no_trace";
+
 val wrapper : (Proof.context -> Method.method) context_parser =
-  (Scan.lift (Scan.option (Args.parens Parse.nat)) -- Method.text_closure)
-  >> (fn (n, text) => method_wrapper n (fn ctxt => Method.evaluate_runtime text ctxt))
+  (Scan.lift (
+    Args.parens Parse.nat >> (fn n => (SOME n, true)) || 
+    Args.parens (Parse.nat -- Args.$$$ no_traceN) >> (fn (n, _) => (SOME n, false)) ||
+    Args.parens (Args.$$$ no_traceN) >> (fn _ => (NONE, false)) ||
+    Scan.succeed (NONE, true)) -- 
+  Method.text_closure)
+  >> (fn ((n, do_trace), text) =>
+    method_wrapper n do_trace (fn ctxt => Method.evaluate_runtime text ctxt))
 
 fun simpT_method meth =
   Scan.lift simp_options --|
     Method.sections Simplifier.simp_modifiers' >>
-    (fn (n, tac) => method_wrapper n (fn ctxt => METHOD (fn facts => meth ctxt tac facts)))
+    (fn (n, tac) => method_wrapper n true (fn ctxt => METHOD (fn facts => meth ctxt tac facts)))
 
 val simp_wrapper =
   simpT_method (fn ctxt => fn tac => fn facts =>
@@ -187,9 +303,9 @@ val auto_wrapper =
     Scan.lift (Scan.option (Parse.nat -- Parse.nat))) --|
     Method.sections clasimp_modifiers >>
   (fn (i, NONE) => 
-      method_wrapper i (SIMPLE_METHOD o CHANGED_PROP o auto_tac)
+      method_wrapper i true (SIMPLE_METHOD o CHANGED_PROP o auto_tac)
     | (i, SOME (m, n)) => 
-      method_wrapper i (fn ctxt => SIMPLE_METHOD (CHANGED_PROP (mk_auto_tac ctxt m n))));
+      method_wrapper i true (fn ctxt => SIMPLE_METHOD (CHANGED_PROP (mk_auto_tac ctxt m n))));
 
 end
 
