thys/AutoCorres2/tests/c-parser/padding_free.thy
@@ -1,0 +1,18 @@
+(*
+ * Copyright (c) 2024 Apple Inc. All rights reserved.
+ *
+ * SPDX-License-Identifier: BSD-2-Clause
+ *)
+
+theory padding_free
+imports "AutoCorres2.CTranslation"
+begin
+
+install_C_file "padding_free.c"
+
+text \<open>Ensure that these types are padding-free (\<^typ>\<open>'a::packed_type\<close>):\<close>
+thm packed_type_access_ti[where 'a=p_t_C]
+thm packed_type_access_ti[where 'a=q_t_C]
+thm packed_type_access_ti[where 'a=r_t_C]
+
+end
