thys/AutoCorres2/tests/proof-tests/Nested_Field_Update.thy
@@ -1,0 +1,80 @@
+(*
+ * Copyright (c) 2024 Apple Inc. All rights reserved.
+ *
+ * SPDX-License-Identifier: BSD-2-Clause
+ *)
+
+theory Nested_Field_Update
+imports "AutoCorres2_Main.AutoCorres_Main"
+begin
+
+record XX =
+ fld1::nat
+ fld2::int
+print_theorems
+install_C_file "nested_field_update.c"
+autocorres "nested_field_update.c"
+
+thm componets_C_idupdates
+thm cs_C_update_def c2_C_update_def recursive_records_fold_congs
+
+thm globals_C_idupdates
+lemma foo: "globals_C (f (cs_C r)) = cs_C_update f r"
+  by (simp cong: recursive_records_fold_congs flip: cs_C_update_def)
+
+
+lemma "globals_C (cs_C r) = X"
+  apply (simp add: foo)
+  oops
+thm foo cs_C_update_def
+lemma cs_C_update_const_select_fold: "cs_C_update (\<lambda>_. f (cs_C r)) r = cs_C_update f r"
+  by (cases r) simp
+
+lemma globals_constr_to_updates: "globals_C a = cs_C_update (\<lambda>_. a) undefined"
+  by simp
+
+lemma bar1: "componets_C (f (c1_C r)) (c2_C r) = c1_C_update f r"
+  by (simp cong: recursive_records_fold_congs flip: c1_C_update_def)
+
+lemma bar2: "componets_C (c1_C r) (f (c2_C r)) = c2_C_update f r"
+  by (simp cong: recursive_records_fold_congs flip: c2_C_update_def)
+
+lemma bar_all: "componets_C (f (c1_C r)) (g (c2_C r)) = c2_C_update g (c1_C_update f r)"
+  by (simp cong: recursive_records_fold_congs flip: c2_C_update_def c1_C_update_def)
+
+lemma components_constr_to_updates: "componets_C a b = c2_C_update (\<lambda>_. b) (c1_C_update (\<lambda>_. a) undefined)"
+  by simp
+
+thm componets_C_idupdates
+thm globals_C_idupdates
+lemma c1_C_update_id: "c1_C_update (\<lambda>a. a) r = r" by (cases r) simp
+lemma "componets_C (c1_C r) (f (c2_C r)) = c2_C_update f r"
+  apply (subst bar_all)
+  apply (simp add: c1_C_update_id)
+  done
+lemma "cs_C_update (\<lambda>_. c) x = globals_C c"
+  by simp
+
+lemma cs_C_update_fld: "cs_C_update (\<lambda>_. f (cs_C r)) r = cs_C_update f r"
+  by (simp (*add: cs_C_update_def*) cong: recursive_records_fold_congs)
+
+
+
+context ts_definition_write_globals
+begin
+lemma " (g_''_update (\<lambda>a. globals_C (c2_C_update (\<lambda>a. c_C 0x2B) (cs_C a)))) = g_''_update (cs_C_update (c2_C_update (\<lambda>_. c_C 0x2B)))"
+
+  apply (simp add: foo)
+  done
+(*
+  apply (simp add: cs_C_update_fld cong: state_fold_congs recursive_records_fold_congs  )
+  thm cs_C_update_def [symmetric] recursive_records_fold_congs 
+  apply (simp cong:  recursive_records_fold_congs flip: cs_C_update_def)
+  oops
+*)
+thm ts_def
+lemma "write_globals' \<equiv> modify (g_''_update (cs_C_update (c2_C_update (\<lambda>_. c_C 0x2B))))"
+  unfolding ts_def .
+end
+
+end
